example/timestamp_proof.v
@@ -19,38 +19,35 @@ Record C :=
 Definition has_encoding (encoded:list u8) (args:C) : Prop :=
   encoded = (u32_le args.(hour)) ++ (u32_le args.(minute)) ++ (u32_le args.(second)).
 
-Definition own args_ptr args q : iProp Σ :=
-  "Hargs_hour" ∷ args_ptr ↦[TimeStamp :: "hour"]{q} #args.(hour) ∗
-  "Hargs_minute" ∷ args_ptr ↦[TimeStamp :: "minute"]{q} #args.(minute) ∗
-  "Hargs_second" ∷ args_ptr ↦[TimeStamp :: "second"]{q} #args.(second).
+Definition own (args__v : val) (args__c : C) (dq : dfrac) : iProp Σ :=
+  "%Hown_struct" ∷ ⌜ args__v = (#args__c.(hour), (#args__c.(minute), (#args__c.(second), #())))%V ⌝.
 
-Lemma wp_Encode (args_ptr:loc) (args:C) (pre_sl:Slice.t) (prefix:list u8) q:
+Lemma wp_Encode (args__v : val) (args__c : C) (pre_sl : Slice.t) (prefix : list u8) (dq : dfrac):
   {{{
-        own args_ptr args q ∗
+        own args__v args__c dq ∗
         own_slice pre_sl byteT (DfracOwn 1) prefix
   }}}
-    MarshalTimeStamp #args_ptr (slice_val pre_sl)
+    MarshalTimeStamp args__v (slice_val pre_sl)
   {{{
         enc enc_sl, RET (slice_val enc_sl);
-        ⌜has_encoding enc args⌝ ∗
+        ⌜ has_encoding enc args__c ⌝ ∗
         own_slice enc_sl byteT (DfracOwn 1) (prefix ++ enc) ∗
-        own args_ptr args q
+        own args__v args__c dq
   }}}.
-
 Proof.
   iIntros (?) "H HΦ". iDestruct "H" as "[Hown Hsl]". iNamed "Hown".
-  wp_rec. wp_pures.
+  wp_rec. wp_pures. iUnfold own in "Hown". iNamed "Hown". rewrite Hown_struct.
   wp_apply (wp_ref_to); first by val_ty.
   iIntros (?) "Hptr".
   wp_pures.
 
-  wp_loadField. wp_load. wp_apply (wp_WriteInt32 with "[$Hsl]").
+  wp_load. wp_apply (wp_WriteInt32 with "[$Hsl]").
   iIntros (?) "Hsl". wp_store.
 
-  wp_loadField. wp_load. wp_apply (wp_WriteInt32 with "[$Hsl]").
+  wp_load. wp_apply (wp_WriteInt32 with "[$Hsl]").
   iIntros (?) "Hsl". wp_store.
 
-  wp_loadField. wp_load. wp_apply (wp_WriteInt32 with "[$Hsl]").
+  wp_load. wp_apply (wp_WriteInt32 with "[$Hsl]").
   iIntros (?) "Hsl". wp_store.
 
   wp_load. iApply "HΦ". iModIntro. rewrite -?app_assoc. iFrame.
@@ -64,29 +61,37 @@ Lemma wp_Decode enc enc_sl (args:C) (suffix : list u8) (q : dfrac):
   }}}
     UnmarshalTimeStamp (slice_val enc_sl)
   {{{
-        args_ptr suff_sl, RET (#args_ptr, suff_sl); own args_ptr args (DfracOwn 1) ∗
+        args_v suff_sl, RET (args_v, suff_sl); own args_v args (DfracOwn 1) ∗
                                                     own_slice_small suff_sl byteT q suffix
   }}}.
 
 Proof.
   iIntros (?) "[%Henc Hsl] HΦ". wp_rec.
-  wp_apply wp_allocStruct; first by val_ty.
-  iIntros (?) "Hs". wp_pures.
   wp_apply wp_ref_to; first done.
-  iIntros (?) "Hptr". wp_pures.
-  iDestruct (struct_fields_split with "Hs") as "HH".
-  iNamed "HH". rewrite Henc.
+  iIntros (ls) "Hs". wp_pures.
 
-  wp_load. wp_apply (wp_ReadInt32 with "[$]"). iIntros (?) "Hs".
-  wp_pures. wp_storeField. wp_store.
+  wp_apply wp_ref_of_zero; first done.
+  iIntros (l__hour) "Hhour". wp_pures.
 
-  wp_load. wp_apply (wp_ReadInt32 with "[$]"). iIntros (?) "Hs".
-  wp_pures. wp_storeField. wp_store.
+  wp_apply wp_ref_of_zero; first done.
+  iIntros (l__minute) "Hminute". wp_pures.
 
-  wp_load. wp_apply (wp_ReadInt32 with "[$]"). iIntros (?) "Hs".
-  wp_pures. wp_storeField. wp_store.
+  wp_apply wp_ref_of_zero; first done.
+  iIntros (l__second) "Hsecond". wp_pures.
 
-  wp_load. wp_pures. iApply "HΦ". iModIntro. iFrame.
+  unfold has_encoding in Henc. rewrite Henc.
+
+  wp_load. wp_apply (wp_ReadInt32 with "[$]"). iIntros (?) "Hsl".
+  wp_pures. wp_store. wp_store.
+
+  wp_load. wp_apply (wp_ReadInt32 with "[$]"). iIntros (?) "Hsl".
+  wp_pures. wp_store. wp_store.
+
+  wp_load. wp_apply (wp_ReadInt32 with "[$]"). iIntros (?) "Hsl".
+  wp_pures. wp_store. wp_store.
+
+  wp_load. wp_load. wp_load. wp_load. wp_pures. iApply "HΦ". iModIntro. iFrame.
+  unfold own. iPureIntro. reflexivity.
 Qed.
 
 End TimeStamp.
